theories/product.v
@@ -689,6 +689,7 @@ Proof.
 Qed.
 Global Hint Resolve mod_map_step_s : tstep.
 
+Global Hint Transparent mod_map : tstep.
 Global Hint Transparent mod_product : tstep.
 Global Hint Transparent mod_map_mod : tstep.
 Global Hint Transparent mod_map_fn : tstep.
