theories/state_transform.v
@@ -1,0 +1,71 @@
+Require Export refframe.module.
+Require Import refframe.trefines.
+Require Import refframe.proof_techniques.
+
+(*** state transform *)
+Inductive state_transform_step {EV S} (m : module EV) (R : S → m.(m_state) → Prop) :
+  S → option EV → (S → Prop) → Prop :=
+| StateTransformStep σ σ' e Pσ:
+  m.(m_step) σ' e Pσ →
+  R σ σ' →
+  state_transform_step m R σ e (λ σ'', ∃ σ''', R σ'' σ''' ∧ Pσ σ''').
+
+Definition mod_state_transform {EV S} (m : module EV) (R : S → m.(m_state) → Prop) :=
+  Mod (state_transform_step m R).
+Global Hint Transparent mod_state_transform : tstep.
+
+Lemma mod_state_transform_nil {EV S} (m : module EV) (R : S → m.(m_state) → Prop) σ σ' (Pσ Pσ' : _ → Prop):
+  σ' ~{ m, tnil }~>ₜ Pσ' →
+  R σ σ' →
+  (∀ σ σ', Pσ' σ' → R σ σ' → Pσ σ) →
+  σ ~{ mod_state_transform m R, tnil }~>ₜ Pσ.
+Proof.
+  move => /thas_trace_nil_inv. have : @tnil EV ⊆ tnil by done. move: {1 3}(tnil) => κs Hnil Ht.
+  elim: Ht σ Pσ Hnil; clear. { tend. naive_solver. }
+  move => σ' Pσ' Pσ'' κ κs κs' Hstep ? IH Hsub σ Pσ Hnil HR Hend. rewrite -Hsub in Hnil.
+  destruct κ; [by inversion Hnil|]; simplify_eq/=.
+  tstep_None; [by econs|] => ?/=[?[??]].
+  apply: IH; naive_solver.
+Qed.
+
+Lemma mod_state_transform_trefines {EV S1 S2} (m1 m2 : module EV) (R1 : S1 → m1.(m_state) → Prop) (R2 : S2 → m2.(m_state) → Prop) σ1' σ1 σ2 σ2':
+  (∀ σ1 σ σ', R1 σ1 σ → R1 σ1 σ' → σ = σ') →
+  (∀ σ1 σ σ' κ Pσ, m_step m1 σ κ Pσ → Pσ σ' → R1 σ1 σ → ∃ σ'', R1 σ'' σ') →
+  trefines (MS m1 σ1') (MS m2 σ2') →
+  R1 σ1 σ1' →
+  R2 σ2 σ2' →
+  trefines (MS (mod_state_transform m1 R1) σ1) (MS (mod_state_transform m2 R2) σ2).
+Proof.
+  move => Heq Hstep Href HR1 HR2.
+  apply wp_implies_refines => n.
+  move: Href => /wp_complete/(_ n)/=.
+  elim/ti_lt_ind: n σ1 σ2 σ1' σ2' HR1 HR2 => n IH σ1 σ2 σ1' σ2' HR1 HRc2 Hwp.
+  apply Wp_step => Pσ n' κ ??. invert_all @m_step.
+  inversion Hwp as [??? Hwp']; simplify_eq.
+  have ?: σ' = σ1' by naive_solver. subst σ'.
+  have [Pσ' [Ht HPσ]]:= Hwp' _ _ _ ltac:(done) ltac:(done).
+  destruct κ; simplify_eq/=.
+  - move: Ht => /(thas_trace_cons_inv _ _ _)?.
+    apply: (thas_trace_trans tnil); [apply: mod_state_transform_nil; [done..|]|move => ? H'; apply H'].
+    move => ?? [? [? HP']] ?.
+    tstep_Some; [by econs|] => /= ? [?[? /HP'?]].
+    apply: mod_state_transform_nil; [done..|] => ??/HPσ[?[??]]?.
+    have [??]:= Hstep _ _ _ _ _ ltac:(done) ltac:(done) ltac:(done).
+    eexists _. split; [naive_solver|].
+    by apply: IH.
+  - apply: mod_state_transform_nil; [done..|] => ??/HPσ[?[??]]?.
+    have [??]:= Hstep _ _ _ _ _ ltac:(done) ltac:(done) ltac:(done).
+    eexists _. split; [naive_solver|].
+    by apply: IH.
+Qed.
+
+Lemma mod_state_transform_tstep_s {EV S} (m : module EV) (f : S → m.(m_state)) σ P `{!TStepS m (f σ) P} :
+  TStepS (mod_state_transform m (λ σ σ', σ' = f σ)) σ (λ G, P (λ κ P', G κ (λ G', P' (λ σ', ∀ σ, σ' = f σ → G' σ)))).
+Proof.
+  constructor => G /tsteps_proof [κ [? [? HG']]]. split!; [done|] => ? /= /HG'/steps_spec_has_trace_1 Ht.
+  apply steps_spec_has_trace_elim. apply: mod_state_transform_nil; [done..|].
+  move => ?? /= ??; subst. case_match; destruct_all?.
+  - apply: steps_spec_step_end; [by econs|] => /= ? [?[??]]. naive_solver.
+  - apply: steps_spec_end. naive_solver.
+Qed.
+Global Hint Resolve mod_state_transform_tstep_s | 20 : tstep.
